adapting two-watched literals to new organisation

Weidenbach_Book/CDCL_Two_Watched_Literals_Invariant.thy
@@ -28,7 +28,12 @@ lemma mset_raw_init_clss_init_state:
   = mset (map clause N)"
   by (metis (no_types, lifting) init_clss_init_state map_eq_conv map_map o_def clause_def)
 
-interpretation rough_cdcl: state\<^sub>W_ops
+fun reduce_trail_to where
+"reduce_trail_to M1 S =
+  (case S of
+    (TWL_State M N U k C) \<Rightarrow> TWL_State (drop (length M - length M1) M) N U k C)"
+
+interpretation rough_cdcl: abs_state\<^sub>W_ops
     clause
     raw_clss_l "op @"
     "\<lambda>L C. L \<in> set C" "op #" "\<lambda>C. remove1_cond (\<lambda>D. clause D = clause C)"
@@ -42,7 +47,7 @@ interpretation rough_cdcl: state\<^sub>W_ops
     cons_trail tl_trail "\<lambda>C. add_learned_cls (raw_clause C)"
     "\<lambda>C. remove_cls (raw_clause C)"
     update_backtrack_lvl
-    update_conflicting "\<lambda>N. init_state (map raw_clause N)" restart'
+    update_conflicting reduce_trail_to "\<lambda>N. init_state (map raw_clause N)" restart'
   rewrites
     "rough_cdcl.mmset_of_mlit = mmset_of_mlit"
 proof goal_cases
@@ -54,11 +59,11 @@ proof goal_cases
     apply (rule ext)
     apply (rename_tac x)
     apply (case_tac x)
-    apply (simp_all add: state\<^sub>W_ops.mmset_of_mlit.simps[OF H] raw_clause_def clause_def)
+    apply (simp_all add: abs_state\<^sub>W_ops.mmset_of_mlit.simps[OF H] raw_clause_def clause_def)
   done
 qed
 
-interpretation rough_cdcl: state\<^sub>W
+interpretation rough_cdcl: abs_state\<^sub>W
     clause
     raw_clss_l "op @"
     "\<lambda>L C. L \<in> set C" "op #" "\<lambda>C. remove1_cond (\<lambda>D. clause D = clause C)"
@@ -72,31 +77,33 @@ interpretation rough_cdcl: state\<^sub>W
     cons_trail tl_trail "\<lambda>C. add_learned_cls (raw_clause C)"
     "\<lambda>C. remove_cls (raw_clause C)"
     update_backtrack_lvl
-    update_conflicting "\<lambda>N. init_state (map raw_clause N)" restart'
+    update_conflicting reduce_trail_to "\<lambda>N. init_state (map raw_clause N)" restart'
 proof goal_cases
   case 1
-  have stupid_locales: "state\<^sub>W_ops clause raw_clss_l op @ (\<lambda>L C. L \<in> set C) op #
+  have stupid_locales: "abs_state\<^sub>W_ops clause raw_clss_l op @ (\<lambda>L C. L \<in> set C) op #
     (\<lambda>C. remove1_cond (\<lambda>D. clause D = clause C)) mset union_mset_list remove1 raw_clause
     (TWL_Clause [])"
     by unfold_locales
-  have [simp]: "state\<^sub>W_ops.mmset_of_mlit clause = mmset_of_mlit"
+  have [simp]: "abs_state\<^sub>W_ops.mmset_of_mlit clause = mmset_of_mlit"
     apply (rule ext, rename_tac L, case_tac L)
-    by (auto simp: state\<^sub>W_ops.mmset_of_mlit.simps[OF stupid_locales] clause_def
+    by (auto simp: abs_state\<^sub>W_ops.mmset_of_mlit.simps[OF stupid_locales] clause_def
     raw_clause_def)
-  have [simp]: "\<And>S. raw_clss_l (restart_learned S) \<subseteq># rough_cdcl.learned_clss S"
+  have [simp]: "\<And>S. raw_clss_l (restart_learned S) \<subseteq># rough_cdcl.conc_learned_clss S"
     using image_mset_subseteq_mono[OF restart_learned] unfolding mset_map
      by blast
-
+  have H: "\<And>M2 M1 x1. map mmset_of_mlit x1 = M2 @ M1 \<Longrightarrow>
+       map mmset_of_mlit (drop (length x1 - length M1) x1) = M1"
+    by (metis add_diff_cancel_right' append_eq_conv_conj drop_map length_append length_map)
   show H: ?case
     apply unfold_locales
     apply (case_tac "raw_trail S"; case_tac "hd (raw_trail S)")
-    by (simp_all add: add_init_cls_def add_learned_cls_def clause_rewatch clause_watch
+    by (auto simp add: add_init_cls_def add_learned_cls_def clause_rewatch clause_watch
       cons_trail_def remove_cls_def restart'_def tl_trail_def map_tl comp_def
       ac_simps mset_map_removeAll_cond mset_raw_init_clss_init_state
-      clause_def[symmetric])
+      clause_def[symmetric] H split: twl_state.splits)
 qed
 
-interpretation rough_cdcl: conflict_driven_clause_learning\<^sub>W
+interpretation rough_cdcl: abs_conflict_driven_clause_learning\<^sub>W
   clause
   raw_clss_l "op @"
   "\<lambda>L C. L \<in> set C" "op #" "\<lambda>C. remove1_cond (\<lambda>D. clause D = clause C)"
@@ -110,7 +117,7 @@ interpretation rough_cdcl: conflict_driven_clause_learning\<^sub>W
   cons_trail tl_trail "\<lambda>C. add_learned_cls (raw_clause C)"
   "\<lambda>C. remove_cls (raw_clause C)"
   update_backtrack_lvl
-  update_conflicting "\<lambda>N. init_state (map raw_clause N)" restart'
+  update_conflicting reduce_trail_to "\<lambda>N. init_state (map raw_clause N)" restart'
   by unfold_locales
 
 declare local.rough_cdcl.mset_ccls_ccls_of_cls[simp del]
@@ -215,10 +222,15 @@ lemma wf_twl_state_update_backtrack_lvl:
 lemma rough_state_of_twl_update_backtrack_lvl:
   "rough_state_of_twl (update_backtrack_lvl_twl k S) = update_backtrack_lvl k
     (rough_state_of_twl S)"
-  using rough_state_of_twl twl_of_rough_state_inverse wf_twl_state_update_backtrack_lvl by fast
+  using rough_state_of_twl[of S] (* TODO remove explicit instantiation *)
+    twl_of_rough_state_inverse[of "update_backtrack_lvl k (rough_state_of_twl S)"]
+    wf_twl_state_update_backtrack_lvl[of "rough_state_of_twl S" k] by fast
 
 abbreviation update_conflicting_twl where
 "update_conflicting_twl k S \<equiv> twl_of_rough_state (update_conflicting k (rough_state_of_twl S))"
+
+abbreviation reduce_trail_to_twl where
+"reduce_trail_to_twl M1 S \<equiv> twl_of_rough_state (reduce_trail_to M1 (rough_state_of_twl S))"
 
 lemma wf_twl_state_update_conflicting:
   "wf_twl_state S \<Longrightarrow> wf_twl_state (update_conflicting k S)"
@@ -254,7 +266,79 @@ lemma undefined_lit_trail_twl_raw_trail[iff]:
   "undefined_lit (trail_twl S) L \<longleftrightarrow> undefined_lit (raw_trail_twl S) L"
   by (auto simp: defined_lit_map image_image)
 
-sublocale wf_twl: conflict_driven_clause_learning\<^sub>W
+
+lemma wf_twl_reduce_trail_to:
+  assumes "trail S = M2 @ M1" and wf: "wf_twl_state S"
+  shows "wf_twl_state (reduce_trail_to M1 S)"
+proof -
+  obtain M N U k C where S: "S = TWL_State M N U k C"
+    by (cases S)
+  have n_d: "no_dup M"
+    using wf by (auto simp: S comp_def wf_twl_state_def)
+  have M: "M = take (length M - length M1) M @ drop (length M - length M1) M"
+    by auto
+  have [simp]: "no_dup (drop (length M - length M1) M)"
+    using n_d by (metis distinct_drop drop_map)
+  have "\<And>C. C \<in> set (twl.raw_clauses S) \<Longrightarrow> wf_twl_cls (raw_trail S) C"
+    using wf by (auto simp: S comp_def wf_twl_state_def)
+  then show ?thesis
+    unfolding wf_twl_state_def S
+    using wf_twl_cls_append[of "take (length M - length M1) M" "drop (length M - length M1) M",
+      unfolded M[symmetric]]
+    by (simp_all add: n_d twl.raw_clauses_def)
+qed
+
+lemma trail_twl_twl_rough_state_reduce_trail_to:
+  assumes "trail_twl st = M2 @ M1"
+  shows "trail_twl (twl_of_rough_state (reduce_trail_to M1 (rough_state_of_twl st))) = M1"
+proof -
+  have "wf_twl_state (reduce_trail_to M1 (rough_state_of_twl st))"
+    using wf_twl_reduce_trail_to assms by fastforce
+  moreover
+    have "length (trail_twl st) - length M1 = length M2"
+      unfolding assms by auto
+    then have "trail (reduce_trail_to M1 (rough_state_of_twl st)) = M1"
+      apply (cases "rough_state_of_twl st")
+      using assms by (auto simp: drop_map[symmetric])
+  ultimately show ?thesis
+    using twl_of_rough_state_inverse[of "reduce_trail_to M1 (rough_state_of_twl st)"]
+    rough_state_of_twl[of st]
+    by (auto simp add: assms)
+qed
+
+lemma twl_of_rough_state_reduce_trail_to:
+  assumes "trail_twl st = M2 @ M1"
+  shows
+    "raw_init_clss_twl (twl_of_rough_state (reduce_trail_to M1 (rough_state_of_twl st)))
+      = raw_init_clss_twl st" (is "?A") and
+    "raw_learned_clss_twl (twl_of_rough_state (reduce_trail_to M1 (rough_state_of_twl st)))
+      = raw_learned_clss_twl st" (is "?B") and
+    "backtrack_lvl_twl (twl_of_rough_state (reduce_trail_to M1 (rough_state_of_twl st)))
+      = backtrack_lvl_twl st" (is "?C") and
+    "rough_cdcl.conc_conflicting (rough_state_of_twl (twl_of_rough_state
+         (reduce_trail_to M1 (rough_state_of_twl st))))
+      = rough_cdcl.conc_conflicting (rough_state_of_twl st)"  (is "?D")
+proof -
+
+  have "wf_twl_state (reduce_trail_to M1 (rough_state_of_twl st))"
+    using wf_twl_reduce_trail_to assms by fastforce
+  moreover
+    have "length (trail_twl st) - length M1 = length M2"
+      unfolding assms by auto
+    then have
+      "raw_init_clss (reduce_trail_to M1 (rough_state_of_twl st)) = raw_init_clss_twl st"
+      "raw_learned_clss (reduce_trail_to M1 (rough_state_of_twl st)) = raw_learned_clss_twl st"
+      "backtrack_lvl (reduce_trail_to M1 (rough_state_of_twl st)) = backtrack_lvl_twl st"
+      "rough_cdcl.conc_conflicting (reduce_trail_to M1 (rough_state_of_twl st)) =
+        rough_cdcl.conc_conflicting (rough_state_of_twl st)"
+      using assms by (cases "rough_state_of_twl st", auto simp: drop_map[symmetric])+
+  ultimately show ?A ?B ?C ?D
+    using twl_of_rough_state_inverse[of "reduce_trail_to M1 (rough_state_of_twl st)"]
+    rough_state_of_twl[of st]
+    by (auto simp add: assms)
+qed
+
+sublocale wf_twl: abs_conflict_driven_clause_learning\<^sub>W
   clause
   raw_clss_l "op @"
   "\<lambda>L C. L \<in> set C" "op #" "\<lambda>C. remove1_cond (\<lambda>D. clause D = clause C)"
@@ -274,43 +358,44 @@ sublocale wf_twl: conflict_driven_clause_learning\<^sub>W
   "\<lambda>C. remove_cls_twl (raw_clause C)"
   update_backtrack_lvl_twl
   update_conflicting_twl
+  reduce_trail_to_twl
   "\<lambda>N. init_state_twl (map raw_clause N)"
   restart_twl
 proof goal_cases
   case 1
-  have stupid_locales: "state\<^sub>W_ops clause raw_clss_l op @ (\<lambda>L C. L \<in> set C) op #
+  have stupid_locales: "abs_state\<^sub>W_ops clause raw_clss_l op @ (\<lambda>L C. L \<in> set C) op #
     (\<lambda>C. remove1_cond (\<lambda>D. clause D = clause C)) mset union_mset_list remove1 raw_clause
     (TWL_Clause [])"
     by unfold_locales
-  have ugly[simp]: "state\<^sub>W_ops.mmset_of_mlit clause = mmset_of_mlit"
+  have ugly[simp]: "abs_state\<^sub>W_ops.mmset_of_mlit clause = mmset_of_mlit"
     apply (rule ext, rename_tac L, case_tac L)
-    by (auto simp: state\<^sub>W_ops.mmset_of_mlit.simps[OF stupid_locales] clause_def
+    by (auto simp: abs_state\<^sub>W_ops.mmset_of_mlit.simps[OF stupid_locales] clause_def
     raw_clause_def)
-  have [simp]: "\<And>S. raw_clss_l (restart_learned S) \<subseteq># rough_cdcl.learned_clss S"
+  have [simp]: "\<And>S. raw_clss_l (restart_learned S) \<subseteq># rough_cdcl.conc_learned_clss S"
     using image_mset_subseteq_mono[OF restart_learned] unfolding mset_map
      by blast
 
   show H: ?case
     apply unfold_locales
-           using rough_cdcl.hd_raw_trail unfolding ugly apply blast
+           using rough_cdcl.hd_raw_conc_trail unfolding ugly apply blast
          apply (simp_all add: rough_state_of_twl_cons_trail rough_state_of_twl_tl_trail
            rough_state_of_twl_add_init_cls rough_state_of_twl_add_learned_cls
            rough_state_of_twl_remove_cls rough_state_of_twl_update_backtrack_lvl
            rough_state_of_twl_update_conflicting)[7]
-       using rough_cdcl.init_clss_cons_trail rough_cdcl.init_clss_tl_trail
-       rough_cdcl.init_clss_remove_cls
-       rough_cdcl.init_clss_add_learned_cls
-       rough_cdcl.init_clss_update_backtrack_lvl
-       rough_cdcl.init_clss_update_conflicting
+       using rough_cdcl.conc_init_clss_cons_conc_trail rough_cdcl.conc_init_clss_tl_conc_trail
+       rough_cdcl.conc_init_clss_remove_cls
+       rough_cdcl.conc_init_clss_add_conc_learned_cls
+       rough_cdcl.conc_init_clss_update_conc_backtrack_lvl
+       rough_cdcl.conc_init_clss_update_conc_conflicting
        apply (auto simp add: rough_state_of_twl_cons_trail rough_state_of_twl_tl_trail
          rough_state_of_twl_add_init_cls rough_state_of_twl_add_learned_cls
          rough_state_of_twl_remove_cls rough_state_of_twl_update_backtrack_lvl
          rough_state_of_twl_update_conflicting comp_def)[7]
-       using rough_cdcl.learned_clss_cons_trail rough_cdcl.learned_clss_tl_trail
-       rough_cdcl.learned_clss_remove_cls
-       rough_cdcl.learned_clss_add_learned_cls
-       rough_cdcl.learned_clss_update_backtrack_lvl
-       rough_cdcl.learned_clss_update_conflicting
+       using rough_cdcl.conc_learned_clss_cons_conc_trail rough_cdcl.conc_learned_clss_tl_conc_trail
+       rough_cdcl.conc_learned_clss_remove_cls
+       rough_cdcl.conc_learned_clss_add_conc_learned_cls
+       rough_cdcl.conc_learned_clss_update_conc_backtrack_lvl
+       rough_cdcl.conc_learned_clss_update_conc_conflicting
        apply (auto simp add: rough_state_of_twl_cons_trail rough_state_of_twl_tl_trail
          rough_state_of_twl_add_init_cls rough_state_of_twl_add_learned_cls
          rough_state_of_twl_remove_cls rough_state_of_twl_update_backtrack_lvl
@@ -321,8 +406,9 @@ proof goal_cases
         rough_state_of_twl_update_conflicting comp_def)[14]
     using init_clss_init_state apply (auto simp: rough_state_of_twl_init_state
       clause_def_lambda comp_def)[5]
-  using rough_cdcl.init_clss_restart_state rough_cdcl.learned_clss_restart_state
+  using rough_cdcl.conc_init_clss_restart_state rough_cdcl.conc_learned_clss_restart_state
   apply (auto simp: rough_state_of_twl_restart_twl)[5]
+  using trail_twl_twl_rough_state_reduce_trail_to twl_of_rough_state_reduce_trail_to apply fast+
   done
 qed
 
@@ -343,10 +429,9 @@ propagate_twl_rule: "(L, C) \<in> candidates_propagate_twl S \<Longrightarrow>
   propagate_twl S S'"
 
 inductive_cases propagate_twlE: "propagate_twl S T"
-
 lemma propagate_twl_iff_propagate:
-  assumes inv: "wf_twl.cdcl\<^sub>W_all_struct_inv S"
-  shows "wf_twl.propagate S T \<longleftrightarrow> propagate_twl S T" (is "?P \<longleftrightarrow> ?T")
+  assumes inv: "cdcl\<^sub>W_mset.cdcl\<^sub>W_all_struct_inv (wf_twl.state S)"
+  shows "wf_twl.propagate_abs S T \<longleftrightarrow> propagate_twl S T" (is "?P \<longleftrightarrow> ?T")
 proof
   assume ?P
   then obtain L E where
@@ -356,10 +441,10 @@ proof
     tr_CNot: "trail_twl S \<Turnstile>as CNot (remove1_mset L (clause E))" and
     undef_lot[simp]: "undefined_lit (trail_twl S) L" and
     "T \<sim> cons_trail_twl (Propagated L E) S"
-    by (blast elim: wf_twl.propagateE)
+    by (blast elim: wf_twl.propagate_absE)
   have "distinct (raw_clause E)"
-    using inv CL_Clauses unfolding wf_twl.cdcl\<^sub>W_all_struct_inv_def distinct_mset_set_def
-    wf_twl.distinct_cdcl\<^sub>W_state_def wf_twl.raw_clauses_def by (auto simp: clause_def)
+    using inv CL_Clauses unfolding cdcl\<^sub>W_mset.cdcl\<^sub>W_all_struct_inv_def distinct_mset_set_def
+    cdcl\<^sub>W_mset.distinct_cdcl\<^sub>W_state_def wf_twl.raw_clauses_def by (auto simp: clause_def)
   then have X: "remove1_mset L (mset (raw_clause E)) = mset_set (set (raw_clause E) - {L})"
     by (auto simp: multiset_eq_iff raw_clause_def count_mset distinct_filter_eq_if)
   have "(L, E) \<in> candidates_propagate_twl S"
@@ -375,7 +460,7 @@ proof
     apply (rule propagate_twl_rule)
        apply (rule \<open>(L, E) \<in> candidates_propagate_twl S\<close>)
       using \<open>T \<sim> cons_trail_twl (Propagated L E) S\<close>
-      apply (auto simp: \<open>raw_conflicting_twl S = None\<close> wf_twl.state_eq_def)
+      apply (auto simp: \<open>raw_conflicting_twl S = None\<close> cdcl\<^sub>W_mset.state_eq_def)
     done
 next
   assume ?T
@@ -390,21 +475,21 @@ next
     undef: "undefined_lit (trail_twl S) L"
     using LC unfolding candidates_propagate_def wf_twl.raw_clauses_def by auto
   have dist: "distinct (raw_clause C)"
-    using inv C'S unfolding wf_twl.cdcl\<^sub>W_all_struct_inv_def wf_twl.distinct_cdcl\<^sub>W_state_def
+    using inv C'S unfolding cdcl\<^sub>W_mset.cdcl\<^sub>W_all_struct_inv_def cdcl\<^sub>W_mset.distinct_cdcl\<^sub>W_state_def
      distinct_mset_set_def twl.raw_clauses_def by (fastforce simp: clause_def)
   then have C_L_L: "mset_set (set (raw_clause C) - {L}) = clause C - {#L#}"
     by (metis distinct_mset_distinct distinct_mset_minus distinct_mset_set_mset_ident mset_remove1
       set_mset_mset set_remove1_eq clause_def)
 
   show ?P
-    apply (rule wf_twl.propagate_rule[of S C L])
+    apply (rule wf_twl.propagate_abs_rule[of S C L])
         using confl apply auto[]
        using C'S unfolding twl.raw_clauses_def apply (simp add: wf_twl.raw_clauses_def)
        using L unfolding candidates_propagate_def apply (auto simp: raw_clause_def clause_def)[]
       using wf_candidates_propagate_sound[OF _ LC] rough_state_of_twl dist
       apply (simp add: distinct_mset_remove1_All true_annots_true_cls clause_def)
      using undef apply simp
-    using T undef unfolding wf_twl.state_eq_def by auto
+    using T undef unfolding cdcl\<^sub>W_mset.state_eq_def by auto
 qed
 
 no_notation twl.state_eq_twl (infix "\<sim>TWL" 51)
@@ -419,7 +504,7 @@ conflict_twl_rule:
 inductive_cases conflict_twlE: "conflict_twl S T"
 
 lemma conflict_twl_iff_conflict:
-  shows "wf_twl.conflict S T \<longleftrightarrow> conflict_twl S T" (is "?C \<longleftrightarrow> ?T")
+  shows "wf_twl.conflict_abs S T \<longleftrightarrow> conflict_twl S T" (is "?C \<longleftrightarrow> ?T")
 proof
   assume ?C
   then obtain D where
@@ -427,7 +512,7 @@ proof
     D: "D \<in> set (wf_twl.raw_clauses S)" and
     MD: "trail_twl S \<Turnstile>as CNot (clause D)" and
     T: "T \<sim> update_conflicting_twl (Some (raw_clause D)) S"
-    by (elim wf_twl.conflictE)
+    by (elim wf_twl.conflict_absE)
 
   have "D \<in> candidates_conflict_twl S"
     apply (rule wf_candidates_conflict_complete)
@@ -436,7 +521,7 @@ proof
     using MD S by auto
   moreover have "T \<sim> twl_of_rough_state (update_conflicting (Some (raw_clause D))
   (rough_state_of_twl S))"
-    using T unfolding rough_cdcl.state_eq_def wf_twl.state_eq_def by auto
+    using T unfolding cdcl\<^sub>W_mset.state_eq_def by auto
   ultimately show ?T
     using S by (auto intro: conflict_twl_rule)
 next
@@ -452,59 +537,12 @@ next
  moreover have "trail_twl S \<Turnstile>as CNot (clause C)"
     using wf_candidates_conflict_sound[OF _ C] by auto
  ultimately show ?C apply -
-   apply (rule wf_twl.conflict.conflict_rule[of _ C])
-   using confl T unfolding rough_cdcl.state_eq_def by (auto simp del: map_map)
+   apply (rule wf_twl.conflict_abs_rule[of _ C])
+   using confl T unfolding cdcl\<^sub>W_mset.state_eq_def by (auto simp del: map_map)
 qed
 
-inductive cdcl\<^sub>W_twl :: "'v wf_twl \<Rightarrow> 'v wf_twl \<Rightarrow> bool" for S :: "'v wf_twl" where
-propagate: "propagate_twl S S' \<Longrightarrow> cdcl\<^sub>W_twl S S'" |
-conflict: "conflict_twl S S' \<Longrightarrow> cdcl\<^sub>W_twl S S'" |
-other: "wf_twl.cdcl\<^sub>W_o S S' \<Longrightarrow> cdcl\<^sub>W_twl S S'"|
-rf: "wf_twl.cdcl\<^sub>W_rf S S' \<Longrightarrow> cdcl\<^sub>W_twl S S'"
-
-lemma cdcl\<^sub>W_twl_iff_cdcl\<^sub>W:
-  assumes "wf_twl.cdcl\<^sub>W_all_struct_inv S"
-  shows "cdcl\<^sub>W_twl S T \<longleftrightarrow> wf_twl.cdcl\<^sub>W S T"
-  by (simp add: assms wf_twl.cdcl\<^sub>W.simps cdcl\<^sub>W_twl.simps conflict_twl_iff_conflict
-    propagate_twl_iff_propagate del: map_map)
-
-lemma rtranclp_cdcl\<^sub>W_twl_all_struct_inv_inv:
-  assumes "cdcl\<^sub>W_twl\<^sup>*\<^sup>* S T" and "wf_twl.cdcl\<^sub>W_all_struct_inv S"
-  shows "wf_twl.cdcl\<^sub>W_all_struct_inv T"
-  using assms by (induction rule: rtranclp_induct)
-  (simp_all add: cdcl\<^sub>W_twl_iff_cdcl\<^sub>W wf_twl.cdcl\<^sub>W_all_struct_inv_inv del: map_map)
-
-lemma rtranclp_cdcl\<^sub>W_twl_iff_rtranclp_cdcl\<^sub>W:
-  assumes "wf_twl.cdcl\<^sub>W_all_struct_inv S"
-  shows "cdcl\<^sub>W_twl\<^sup>*\<^sup>* S T \<longleftrightarrow> wf_twl.cdcl\<^sub>W\<^sup>*\<^sup>* S T" (is "?T \<longleftrightarrow> ?W")
-proof
-  assume ?W
-  then show ?T
-    proof (induction rule: rtranclp_induct)
-      case base
-      then show ?case by simp
-    next
-      case (step T U) note st = this(1) and cdcl = this(2) and IH = this(3)
-      have "cdcl\<^sub>W_twl T U"
-        using assms st cdcl wf_twl.rtranclp_cdcl\<^sub>W_all_struct_inv_inv cdcl\<^sub>W_twl_iff_cdcl\<^sub>W
-        by blast
-      then show ?case using IH by auto
-    qed
-next
-  assume ?T
-  then show ?W
-    proof (induction rule: rtranclp_induct)
-      case base
-      then show ?case by simp
-    next
-      case (step T U) note st = this(1) and cdcl = this(2) and IH = this(3)
-      have "wf_twl.cdcl\<^sub>W T U"
-        using assms st cdcl rtranclp_cdcl\<^sub>W_twl_all_struct_inv_inv cdcl\<^sub>W_twl_iff_cdcl\<^sub>W
-        by blast
-      then show ?case using IH by auto
-    qed
-qed
-
+text \<open>We have shown that we we can use @{term conflict_twl} and @{term propagate_twl} in a CDCL
+  calculus.\<close>
 end
 
 end
